OCL_Examples.thy
@@ -250,150 +250,431 @@ section \<open>Typing\<close>
 
 subsection \<open>Positive Cases\<close>
 
+
+(*declare normalize_normalize_call_normalize_expr_list.intros [intro!]*)
+(*declare nf_typing.intros [intro!]*)
+
+
+(*
+inductive_simps q52 [simp]: "\<Gamma> \<turnstile> expr : \<tau>"
+inductive_simps q57 [simp]: "\<Gamma> \<turnstile>\<^sub>E BooleanLiteral c : \<tau>"
+inductive_simps q58 [simp]: "\<Gamma> \<turnstile>\<^sub>E NullLiteral : \<tau>"
+inductive_simps q59 [simp]: "\<Gamma> \<turnstile>\<^sub>E IntegerLiteral c : \<tau>"
+inductive_simps q60 [simp]: "\<Gamma> \<turnstile> Var v \<Rrightarrow> expr"
+inductive_simps q61 [simp]: "\<Gamma> \<turnstile>\<^sub>E Var v : \<tau>"
+inductive_simps q62 [simp]: "\<Gamma> \<turnstile>\<^sub>E Let v ty init body : \<tau>"
+inductive_simps q63 [simp]: "\<Gamma> \<turnstile> Let v ty init body \<Rrightarrow> expr"
+*)
+
+(*** Simplification Rules ***************************************************)
+
+section \<open>Simplification Rules\<close>
+(*
+inductive_simps op_type_simp [simp]: "op_type op k \<tau> \<pi> \<sigma>"
+
+inductive_simps unop_type_simp [simp]: "unop_type op k \<tau> \<sigma>"
+inductive_simps binop_type_simp [simp]: "binop_type op k \<tau> \<sigma> \<rho>"
+inductive_simps ternop_type_simp [simp]: "ternop_type op k \<tau> \<sigma> \<rho> \<upsilon>"
+
+inductive_simps any_unop_type_simp [simp]: "any_unop_type op \<tau> \<sigma>"
+inductive_simps boolean_unop_type_simp [simp]: "boolean_unop_type op \<tau> \<sigma>"
+inductive_simps numeric_unop_type_simp [simp]: "numeric_unop_type op \<tau> \<sigma>"
+inductive_simps string_unop_type_simp [simp]: "string_unop_type op \<tau> \<sigma>"
+inductive_simps collection_unop_type_simp [simp]: "collection_unop_type op \<tau> \<sigma>"
+
+inductive_simps super_binop_type_simp [simp]: "super_binop_type op \<tau> \<sigma> \<rho>"
+inductive_simps boolean_binop_type_simp [simp]: "boolean_binop_type op \<tau> \<sigma> \<rho>"
+inductive_simps numeric_binop_type_simp [simp]: "numeric_binop_type op \<tau> \<sigma> \<rho>"
+inductive_simps string_binop_type_simp [simp]: "string_binop_type op \<tau> \<sigma> \<rho>"
+inductive_simps collection_binop_type_simp [simp]: "collection_binop_type op \<tau> \<sigma> \<rho>"
+
+inductive_simps string_ternop_type_simp [simp]: "string_ternop_type op \<tau> \<sigma> \<rho> \<upsilon>"
+inductive_simps collection_ternop_type_simp [simp]: "collection_ternop_type op \<tau> \<sigma> \<rho> \<upsilon>"
+*)
+
+inductive_simps op_type_alt_simps:
+"mataop_type \<tau> op \<sigma>"
+"typeop_type k op \<tau> \<sigma> \<rho>"
+
+"op_type op k \<tau> \<pi> \<sigma>"
+"unop_type op k \<tau> \<sigma>"
+"binop_type op k \<tau> \<sigma> \<rho>"
+"ternop_type op k \<tau> \<sigma> \<rho> \<upsilon>"
+
+"any_unop_type op \<tau> \<sigma>"
+"boolean_unop_type op \<tau> \<sigma>"
+"numeric_unop_type op \<tau> \<sigma>"
+"string_unop_type op \<tau> \<sigma>"
+"collection_unop_type op \<tau> \<sigma>"
+
+"super_binop_type op \<tau> \<sigma> \<rho>"
+"boolean_binop_type op \<tau> \<sigma> \<rho>"
+"numeric_binop_type op \<tau> \<sigma> \<rho>"
+"string_binop_type op \<tau> \<sigma> \<rho>"
+"collection_binop_type op \<tau> \<sigma> \<rho>"
+
+"string_ternop_type op \<tau> \<sigma> \<rho> \<upsilon>"
+"collection_ternop_type op \<tau> \<sigma> \<rho> \<upsilon>"
+
+
+(*
+declare boolean_unop_type.intros [intro!]
+declare numeric_unop_type.intros [intro!]
+declare string_unop_type.intros [intro!]
+declare collection_unop_type.intros [intro!]
+
+declare op_type.intros [intro!]
+
+declare unop_type.intros [intro!]
+declare binop_type.intros [intro!]
+declare ternop_type.intros [intro!]
+
+declare any_unop_type.intros [intro!]
+declare boolean_unop_type.intros [intro!]
+declare numeric_unop_type.intros [intro!]
+declare string_unop_type.intros [intro!]
+declare collection_unop_type.intros [intro!]
+
+declare super_binop_type.intros [intro!]
+declare boolean_binop_type.intros [intro!]
+declare numeric_binop_type.intros [intro!]
+declare string_binop_type.intros [intro!]
+declare collection_binop_type.intros [intro!]
+
+declare string_ternop_type.intros [intro!]
+declare collection_ternop_type.intros [intro!]
+*)
+
+
+
+print_theorems
+(*
+inductive_simps q64 [simp]: "\<Gamma> \<turnstile>\<^sub>E OperationCall src k op params : \<tau>"
+inductive_simps q65 [simp]: "\<Gamma> \<turnstile>\<^sub>L [] : \<tau>"
+inductive_simps q66 [simp]: "\<Gamma> \<turnstile>\<^sub>L x # xs : \<tau>"
+inductive_simps q70 [simp]: "\<Gamma> \<turnstile>\<^sub>E Var v : \<tau>"
+inductive_simps q71 [simp]: "\<Gamma> \<turnstile>\<^sub>E Let v ty init body : \<tau>"
+inductive_simps q72 [simp]: "\<Gamma> \<turnstile>\<^sub>E CollectionLiteral k prts : \<tau>"
+inductive_simps q73 [simp]: "\<Gamma> \<turnstile>\<^sub>C [x] : \<tau>"
+inductive_simps q74 [simp]: "\<Gamma> \<turnstile>\<^sub>C x # y # xs : \<tau>"
+inductive_simps q75 [simp]: "\<Gamma> \<turnstile>\<^sub>P CollectionItem a : \<tau>"
+inductive_simps q76 [simp]: "\<Gamma> \<turnstile>\<^sub>P CollectionRange a b : \<tau>"
+*)
+(*
+inductive_simps q54 [simp]: "\<Gamma> \<turnstile>\<^sub>C Operation op params \<Rrightarrow> expr"
+inductive_simps q55 [simp]: "\<Gamma> \<turnstile>\<^sub>L [] \<Rrightarrow> expr"
+inductive_simps q56 [simp]: "\<Gamma> \<turnstile>\<^sub>L x # xs \<Rrightarrow> expr"
+
+inductive_simps q50 [simp]: "\<Gamma> \<turnstile> OperationCall src k op params \<Rrightarrow> \<tau>"
+inductive_simps q53 [simp]: "\<Gamma> \<turnstile> Literal c \<Rrightarrow> expr"
+inductive_simps q68 [simp]: "\<Gamma> \<turnstile> Let v ty init body \<Rrightarrow> expr"
+inductive_simps q69 [simp]: "\<Gamma> \<turnstile> Var v \<Rrightarrow> expr"
+*)
+(*
+inductive_simps q51 [simp]: "element_type \<tau> \<sigma>"
+inductive_simps q67 [simp]: "\<Gamma> \<turnstile> expr : \<tau>"
+*)
+inductive_simps typing_alt_simps: 
+"\<Gamma> \<turnstile>\<^sub>E NullLiteral : \<tau>"
+"\<Gamma> \<turnstile>\<^sub>E BooleanLiteral c : \<tau>"
+"\<Gamma> \<turnstile>\<^sub>E RealLiteral c : \<tau>"
+"\<Gamma> \<turnstile>\<^sub>E UnlimitedNaturalLiteral c : \<tau>"
+"\<Gamma> \<turnstile>\<^sub>E IntegerLiteral c : \<tau>"
+"\<Gamma> \<turnstile>\<^sub>E StringLiteral c : \<tau>"
+"\<Gamma> \<turnstile>\<^sub>E EnumLiteral enm lit : \<tau>"
+"\<Gamma> \<turnstile>\<^sub>E CollectionLiteral k prts : \<tau>"
+"\<Gamma> \<turnstile>\<^sub>E TupleLiteral [] : \<tau>"
+"\<Gamma> \<turnstile>\<^sub>E TupleLiteral (x # xs) : \<tau>"
+
+"\<Gamma> \<turnstile>\<^sub>E Let v \<tau> init body : \<sigma>"
+"\<Gamma> \<turnstile>\<^sub>E Var v : \<tau>"
+"\<Gamma> \<turnstile>\<^sub>E If a b c : \<tau>"
+
+"\<Gamma> \<turnstile>\<^sub>E MetaOperationCall \<tau> op : \<sigma>"
+"\<Gamma> \<turnstile>\<^sub>E StaticOperationCall \<tau> op as : \<sigma>"
+
+"\<Gamma> \<turnstile>\<^sub>E TypeOperationCall a k op \<sigma> : \<tau>"
+"\<Gamma> \<turnstile>\<^sub>E AttributeCall src k prop : \<tau>"
+"\<Gamma> \<turnstile>\<^sub>E AssociationEndCall src k role from : \<tau>"
+"\<Gamma> \<turnstile>\<^sub>E AssociationClassCall src k a from : \<tau>"
+"\<Gamma> \<turnstile>\<^sub>E AssociationClassEndCall src k role : \<tau>"
+"\<Gamma> \<turnstile>\<^sub>E OperationCall src k op params : \<tau>"
+"\<Gamma> \<turnstile>\<^sub>E TupleElementCall src k elem : \<tau>"
+
+"\<Gamma> \<turnstile>\<^sub>I (src, its, body) : ys"
+"\<Gamma> \<turnstile>\<^sub>E IterateCall src k its its_ty res res_t res_init body : \<tau>"
+"\<Gamma> \<turnstile>\<^sub>E AnyIteratorCall src k its its_ty body : \<tau>"
+"\<Gamma> \<turnstile>\<^sub>E ClosureIteratorCall src k its its_ty body : \<tau>"
+"\<Gamma> \<turnstile>\<^sub>E CollectIteratorCall src k its its_ty body : \<tau>"
+"\<Gamma> \<turnstile>\<^sub>E CollectNestedIteratorCall src k its its_ty body : \<tau>"
+"\<Gamma> \<turnstile>\<^sub>E ExistsIteratorCall src k its its_ty body : \<tau>"
+"\<Gamma> \<turnstile>\<^sub>E ForAllIteratorCall src k its its_ty body : \<tau>"
+"\<Gamma> \<turnstile>\<^sub>E OneIteratorCall src k its its_ty body : \<tau>"
+"\<Gamma> \<turnstile>\<^sub>E IsUniqueIteratorCall src k its its_ty body : \<tau>"
+"\<Gamma> \<turnstile>\<^sub>E SelectIteratorCall src k its its_ty body : \<tau>"
+"\<Gamma> \<turnstile>\<^sub>E RejectIteratorCall src k its its_ty body : \<tau>"
+"\<Gamma> \<turnstile>\<^sub>E SortedByIteratorCall src k its its_ty body : \<tau>"
+
+"\<Gamma> \<turnstile>\<^sub>C [x] : \<tau>"
+"\<Gamma> \<turnstile>\<^sub>C x # y # xs : \<tau>"
+"\<Gamma> \<turnstile>\<^sub>P CollectionItem a : \<tau>"
+"\<Gamma> \<turnstile>\<^sub>P CollectionRange a b : \<tau>"
+"\<Gamma> \<turnstile>\<^sub>L [] : \<pi>"
+"\<Gamma> \<turnstile>\<^sub>L x # xs : \<pi>"
+
+inductive_simps normalize_alt_simps:
+"\<Gamma> \<turnstile> Literal a \<Rrightarrow> b"
+"\<Gamma> \<turnstile> Let v t init body \<Rrightarrow> b"
+"\<Gamma> \<turnstile> Var v \<Rrightarrow> b"
+"\<Gamma> \<turnstile> If a b c \<Rrightarrow> d"
+
+"\<Gamma> \<turnstile> MetaOperationCall \<tau> op \<Rrightarrow> b"
+"\<Gamma> \<turnstile> StaticOperationCall \<tau> op as \<Rrightarrow> b"
+"\<Gamma> \<turnstile> Call src DotCall call \<Rrightarrow> b"
+"\<Gamma> \<turnstile> Call src SafeDotCall call \<Rrightarrow> b"
+"\<Gamma> \<turnstile> Call src ArrowCall call \<Rrightarrow> b"
+"\<Gamma> \<turnstile> Call src SafeArrowCall call \<Rrightarrow> b"
+
+"(\<Gamma>, \<tau>) \<turnstile>\<^sub>C call \<Rrightarrow> b"
+"(\<Gamma>, \<tau>) \<turnstile>\<^sub>C Operation op as \<Rrightarrow> call"
+"(\<Gamma>, \<tau>) \<turnstile>\<^sub>C Iterate its its_ty res res_t res_init body \<Rrightarrow> call"
+"(\<Gamma>, \<tau>) \<turnstile>\<^sub>C Iterator iter its its_ty body \<Rrightarrow> call"
+
+"\<Gamma> \<turnstile>\<^sub>L [] \<Rrightarrow> ys"
+"\<Gamma> \<turnstile>\<^sub>L x # xs \<Rrightarrow> ys"
+
+(*
+declare op_type.intros [intro!]
+declare binop_type.intros [intro!]
+declare boolean_binop_type.intros [intro!]
+*)
+print_theorems
+
+declare nf_typing.simps [simp]
+
+declare op_type_alt_simps [simp]
+declare typing_alt_simps [simp]
+declare normalize_alt_simps [simp]
+
+declare element_type.simps [simp]
+declare update_element_type.simps [simp]
+declare to_unique_collection.simps [simp]
+declare to_nonunique_collection.simps [simp]
+declare to_ordered_collection.simps [simp]
+
+
+abbreviation "\<Gamma> \<equiv> fmempty :: classes1 type env"
+
 text \<open>
 \<^verbatim>\<open>E1::A : E1[1]\<close>\<close>
-values "{x. (fmempty :: classes1 type env) \<turnstile>
-  EnumLiteral STR ''E1'' STR ''A'' : x}"
+lemma
+  "\<Gamma> \<turnstile> EnumLiteral STR ''E1'' STR ''A'' : (Enum STR ''E1'')[1]"
+  by (auto simp add: literals_classes1_def)
 
 text \<open>
 \<^verbatim>\<open>true or false : Boolean[1]\<close>\<close>
-values "{x. (fmempty :: classes1 type env) \<turnstile>
-  OperationCall (BooleanLiteral True) DotCall OrOp [BooleanLiteral False] : x}"
+lemma
+  "\<Gamma> \<turnstile>
+    OperationCall (BooleanLiteral True) DotCall OrOp
+      [BooleanLiteral False] : Boolean[1]"
+  by auto
 
 text \<open>
 \<^verbatim>\<open>null and true : Boolean[?]\<close>\<close>
-values "{x. (fmempty :: classes1 type env) \<turnstile>
-  OperationCall (NullLiteral) DotCall AndOp [BooleanLiteral True] : x}"
+lemma
+  "\<Gamma> \<turnstile>
+    OperationCall (NullLiteral) DotCall AndOp
+      [BooleanLiteral True] : Boolean[?]"
+  by auto
 
 text \<open>
 \<^verbatim>\<open>let x : Real[1] = 5 in x + 7 : Real[1]\<close>\<close>
-values "{x. (fmempty :: classes1 type env) \<turnstile>
-  Let (STR ''x'') (Some Real[1]) (IntegerLiteral 5)
-    (OperationCall (Var STR ''x'') DotCall PlusOp [IntegerLiteral 7]) : x}"
+lemma
+  "\<Gamma> \<turnstile>
+    Let (STR ''x'') (Some Real[1]) (IntegerLiteral 5)
+    (OperationCall (Var STR ''x'') DotCall PlusOp [IntegerLiteral 7]) : Real[1]"
+  by auto
 
 text \<open>
 \<^verbatim>\<open>null.oclIsUndefined() : Boolean[1]\<close>\<close>
-values "{x. (fmempty :: classes1 type env) \<turnstile>
-  OperationCall (NullLiteral) DotCall OclIsUndefinedOp [] : x}"
+lemma
+  "\<Gamma> \<turnstile>
+    OperationCall (NullLiteral) DotCall OclIsUndefinedOp [] : Boolean[1]"
+  by auto
+
+(*
+declare element_type.intros [intro!]
+declare to_nonunique_collection.intros [intro!]
+declare update_element_type.intros [intro!]
+*)
+
+lemma q81 [simp]:
+  "Sequence \<tau> \<le> OclAny[?] = False"
+  by auto
+
+lemma q82 [simp]:
+  "Sequence \<tau> \<le> Tuple \<pi> = False"
+  by auto
 
 text \<open>
 \<^verbatim>\<open>Sequence{1..5, null}.oclIsUndefined() : Sequence(Boolean[1])\<close>\<close>
-values "{x. (fmempty :: classes1 type env) \<turnstile>
-  OperationCall (CollectionLiteral SequenceKind
+lemma
+  "\<Gamma> \<turnstile>
+    OperationCall (CollectionLiteral SequenceKind
               [CollectionRange (IntegerLiteral 1) (IntegerLiteral 5),
                CollectionItem NullLiteral])
-    DotCall OclIsUndefinedOp [] : x}"
+    DotCall OclIsUndefinedOp [] : Sequence Boolean[1]"
+  by auto
 
 text \<open>
 \<^verbatim>\<open>Sequence{1..5}->product(Set{'a', 'b'})
   : Set(Tuple(first: Integer[1], second: String[1]))\<close>\<close>
-values "{x. (fmempty :: classes1 type env) \<turnstile>
-  OperationCall
-    (CollectionLiteral SequenceKind
+lemma
+  "\<Gamma> \<turnstile>
+    OperationCall (CollectionLiteral SequenceKind
       [CollectionRange (IntegerLiteral 1) (IntegerLiteral 5)])
-    ArrowCall
-    ProductOp
-    [CollectionLiteral SetKind
-      [CollectionItem (StringLiteral ''a''), CollectionItem (StringLiteral ''b'')]] : x}"
+      ArrowCall ProductOp
+      [CollectionLiteral SetKind
+        [CollectionItem (StringLiteral ''a''),
+         CollectionItem (StringLiteral ''b'')]] :
+    Set (Tuple (fmap_of_list [(STR ''first'', Integer[1]), (STR ''second'', String[1])]))"
+  by auto
 
+
+lemma q83 [simp]:
+  "\<tau>[1] < \<tau>[?]"
+  "\<tau>[1] \<le> \<tau>[?]"
+  apply auto
+  by (simp add: less_type_def subtype.intros(3) tranclp.r_into_trancl)
+(*
+declare update_element_type.intros [intro]
+declare update_element_type.simps [simp]
+*)
 text \<open>
 \<^verbatim>\<open>Sequence{1..5, null}?->iterate(x, acc : Real[1] = 0 | acc + x)
   : Real[1]\<close>\<close>
-values "{x. (fmempty :: classes1 type env) \<turnstile>
-  IterateCall (CollectionLiteral SequenceKind
+lemma
+  "\<Gamma> \<turnstile>
+    IterateCall (CollectionLiteral SequenceKind
               [CollectionRange (IntegerLiteral 1) (IntegerLiteral 5),
                CollectionItem NullLiteral]) SafeArrowCall
       [STR ''x''] None
       (STR ''acc'') (Some Real[1]) (IntegerLiteral 0)
-    (OperationCall (Var STR ''acc'') DotCall PlusOp [Var STR ''x'']) : x}"
+    (OperationCall (Var STR ''acc'') DotCall PlusOp [Var STR ''x'']) : Real[1]"
+  by auto
 
 text \<open>
 \<^verbatim>\<open>Sequence{1..5, null}?->max() : Integer[1]\<close>\<close>
-values "{x. (fmempty :: classes1 type env) \<turnstile>
-  OperationCall (CollectionLiteral SequenceKind
+lemma
+  "\<Gamma> \<turnstile>
+    OperationCall (CollectionLiteral SequenceKind
               [CollectionRange (IntegerLiteral 1) (IntegerLiteral 5),
                CollectionItem NullLiteral])
-      SafeArrowCall CollectionMaxOp [] : x}"
+      SafeArrowCall CollectionMaxOp [] : Integer[1]"
+  by auto
 
 text \<open>
 \<^verbatim>\<open>let x : Sequence(String[?]) = Sequence{'abc', 'zxc'} in
 x->any(it | it = 'test') : String[?]\<close>\<close>
-values "{x. (fmempty :: classes1 type env) \<turnstile>
+lemma
+  "\<Gamma> \<turnstile>
   Let (STR ''x'') (Some (Sequence String[?])) (CollectionLiteral SequenceKind
     [CollectionItem (StringLiteral ''abc''),
      CollectionItem (StringLiteral ''zxc'')])
   (AnyIteratorCall (Var STR ''x'') ArrowCall [STR ''it''] (Some String[?])
-    (OperationCall (Var STR ''it'') DotCall EqualOp [StringLiteral ''test''])) : x}"
+    (OperationCall (Var STR ''it'') DotCall EqualOp [StringLiteral ''test''])) : String[?]"
+  by auto
 
 text \<open>
 \<^verbatim>\<open>let x : Sequence(String[?]) = Sequence{'abc', 'zxc'} in
 x?->closure(it | it) : OrderedSet(String[1])\<close>\<close>
-values "{x. (fmempty :: classes1 type env) \<turnstile>
+lemma
+  "\<Gamma> \<turnstile>
   Let STR ''x'' (Some (Sequence String[?])) (CollectionLiteral SequenceKind
     [CollectionItem (StringLiteral ''abc''),
      CollectionItem (StringLiteral ''zxc'')])
   (ClosureIteratorCall (Var STR ''x'') SafeArrowCall [STR ''it''] None
-    (Var STR ''it'')) : x}"
+    (Var STR ''it'')) : OrderedSet String[1]"
+  by auto
+
+lemma q [simp]:
+  "(Employee \<le> \<tau>) = (\<tau> = Employee \<or> \<tau> = Person \<or> \<tau> = Object)"
+  by (metis dual_order.order_iff_strict less_classes1_def subclass1.simps)
 
 text \<open>
 \<^verbatim>\<open>context Employee:
 name : String[1]\<close>\<close>
-values "{x. (fmap_of_list [(STR ''self'', Employee[1])] :: classes1 type env) \<turnstile>
-  AttributeCall (Var STR ''self'') DotCall STR ''name'' : x}"
+lemma
+  "\<Gamma>(STR ''self'' \<mapsto>\<^sub>f Employee[1]) \<turnstile>
+    AttributeCall (Var STR ''self'') DotCall STR ''name'' : String[1]"
+  apply (auto simp add: attributes_classes1_def)
 
 text \<open>
 \<^verbatim>\<open>context Employee:
 projects : Set(Project[1])\<close>\<close>
-values "{x. (fmap_of_list [(STR ''self'', Employee[1])] :: classes1 type env) \<turnstile>
-  AssociationEndCall (Var STR ''self'') DotCall STR ''projects'' None : x}"
+lemma
+  "\<Gamma>(STR ''self'' \<mapsto>\<^sub>f Employee[1]) \<turnstile>
+    AssociationEndCall (Var STR ''self'') DotCall STR ''projects'' None : Set Project[1]"
+  apply auto
 
 text \<open>
 \<^verbatim>\<open>context Employee:
 projects.members : Bag(Employee[1])\<close>\<close>
-values "{x. (fmap_of_list [(STR ''self'', Employee[1])] :: classes1 type env) \<turnstile>
+lemma
+  "\<Gamma>(STR ''self'' \<mapsto>\<^sub>f Employee[1]) \<turnstile>
   AssociationEndCall (AssociationEndCall (Var STR ''self'')
       DotCall STR ''projects'' None)
-    DotCall STR ''members'' None : x}"
+    DotCall STR ''members'' None : Bag Employee[1]"
+  apply simp
 
 text \<open>
 \<^verbatim>\<open>Project[?].allInstances() : Set(Project[?])\<close>\<close>
-values "{x. (fmempty :: classes1 type env) \<turnstile>
-  MetaOperationCall Project[?] AllInstancesOp : x}"
+lemma
+  "\<Gamma> \<turnstile> MetaOperationCall Project[?] AllInstancesOp : Set Project[?]"
+  by auto
 
 text \<open>
 \<^verbatim>\<open>Project[1]::allProjects() : Set(Project[1])\<close>\<close>
-values "{x. (fmempty :: classes1 type env) \<turnstile>
-  StaticOperationCall Project[1] STR ''allProjects'' [] : x}"
+lemma
+  "\<Gamma> \<turnstile> StaticOperationCall Project[1] STR ''allProjects'' [] : Set Project[1]"
+  apply auto
 
 subsection \<open>Negative Cases\<close>
 
 text \<open>
 \<^verbatim>\<open>true = null\<close>\<close>
-values "{x. (fmempty :: classes1 type env) \<turnstile>
-  OperationCall (BooleanLiteral True) DotCall EqualOp [NullLiteral] : x}"
+lemma
+  "\<nexists>\<tau>. \<Gamma> \<turnstile> OperationCall (BooleanLiteral True) DotCall EqualOp [NullLiteral] : \<tau>"
+  by auto
 
 text \<open>
 \<^verbatim>\<open>let x : Boolean[1] = 5 in x and true\<close>\<close>
-values "{x. (fmempty :: classes1 type env) \<turnstile>
-  Let STR ''x'' (Some Boolean[1]) (IntegerLiteral 5)
-    (OperationCall (Var STR ''x'') DotCall AndOp [BooleanLiteral True]) : x}"
+lemma
+  "\<nexists>\<tau>. \<Gamma> \<turnstile>
+    Let STR ''x'' (Some Boolean[1]) (IntegerLiteral 5)
+      (OperationCall (Var STR ''x'') DotCall AndOp [BooleanLiteral True]) : \<tau>"
+  by auto
 
 text \<open>
 \<^verbatim>\<open>let x : Sequence String[?] = Sequence{'abc', 'zxc'} in
 x->closure(it | 1)\<close>\<close>
-values "{x. (fmempty :: classes1 type env) \<turnstile>
-  Let STR ''x'' (Some (Sequence String[?])) (CollectionLiteral SequenceKind
-    [CollectionItem (StringLiteral ''abc''),
-     CollectionItem (StringLiteral ''zxc'')])
-  (ClosureIteratorCall (Var STR ''x'') ArrowCall [STR ''it''] None
-    (IntegerLiteral 1)) : x}"
+lemma
+  "\<nexists>\<tau>. \<Gamma> \<turnstile>
+    Let STR ''x'' (Some (Sequence String[?])) (CollectionLiteral SequenceKind
+      [CollectionItem (StringLiteral ''abc''),
+       CollectionItem (StringLiteral ''zxc'')])
+    (ClosureIteratorCall (Var STR ''x'') ArrowCall [STR ''it''] None
+      (IntegerLiteral 1)) : \<tau>"
+  by auto
 
 text \<open>
 \<^verbatim>\<open>Sequence{1..5, null}->max()\<close>\<close>
-values "{x. (fmempty :: classes1 type env) \<turnstile>
-  OperationCall (CollectionLiteral SequenceKind
-              [CollectionRange (IntegerLiteral 1) (IntegerLiteral 5),
-               CollectionItem NullLiteral])
-      ArrowCall CollectionMaxOp [] : x}"
+lemma
+  "\<nexists>\<tau>. \<Gamma> \<turnstile>
+    OperationCall (CollectionLiteral SequenceKind
+                [CollectionRange (IntegerLiteral 1) (IntegerLiteral 5),
+                 CollectionItem NullLiteral])
+        ArrowCall CollectionMaxOp [] : \<tau>"
+  apply auto
 
 end
